\newpage
\section{Derivative Cheat Sheet}
\begin{multicols}{2}
\begin{align*}
&(y = c)\to y' = 0 \\
&(ax^n)' = a(x^n)' = anx^{n-1} \\
&(u \pm v)' = u' \pm v' \\
&(uv)' = u'v + uv' \\
&(au^n)' = a(u^n)' = anu^{n-1}u' \\
&(\frac{u}{v})' = \frac{u'v - uv'}{v^2} \to (\frac{1}{x})' = \frac{-1}{x^2} \\
&(\sqrt{u})' = \frac{u'}{2\sqrt{u}} \to (\sqrt{x})' = \frac{1}{2\sqrt{x}} \\
&(\ln u)' = \frac{u'}{u} \to (\ln x)' = \frac{1}{x}  \\
&(a^u)' \overset{a>0}{\longrightarrow} u'a^u\ln a \to (a^x)' = a^x\ln a \\
&(e^u)' = u'e^u\ln e = u'e^u \to (e^{ax+b})' = ae^{ax+b} \\
&(u^v)' \overset{u>0}{\longrightarrow} u^v(v'\ln u+\frac{u'v}{u}) \to (x^x)' = (1 + \ln x) \\
&(\sin u)' = u'\cos u \longrightarrow (sin(ax+b))' = a \cos(ax+b) \longrightarrow (\sin x)' = \cos x \\
&(\tan u)' = u'(1+\tan^2u) = u'\sec^2u \to (\tan x)' = 1+\tan^2 x = \sec^2 x \\
&(\cot u)' = -u'(1+\cot^2u) = -u'csc^2u \to (\cot x)' = -(1+\cot^2x) = -csc^2x \\
&(\sec u)' = u'\sec u \tan u \to (sec x)' = x'\sec x\tan x \\
& (csc u)' = -u'.\csc u.\cot u \to (\csc x)' = -\cot x.\csc x \\
\end{align*}

\end{multicols}